more

Weidenbach_Book/IsaSAT_CDCL.thy
@@ -574,16 +574,111 @@ prepare_code_thms (in -) cdcl_twl_stgy_prog_wl_D_code_def
 
 lemmas cdcl_twl_stgy_prog_wl_D_code[sepref_fr_rules] =
    cdcl_twl_stgy_prog_wl_D_code.refine[of \<A>\<^sub>i\<^sub>n]
+end
 
+definition (in -)isasat_fast2 where
+  \<open>isasat_fast2 = isasat_fast\<close>
+
+
+definition (in -) isasat_fast_clss :: \<open>_ \<Rightarrow> bool\<close> where
+  \<open>isasat_fast_clss = (\<lambda>N. length N \<le> uint32_max)\<close>
+
+definition (in -) isasat_fast_clss_dom :: \<open>_ \<Rightarrow> bool\<close> where
+  \<open>isasat_fast_clss_dom = (\<lambda>N. \<forall>L\<in>#dom_m N. L < uint32_max)\<close>
+
+
+lemma (in -) isasat_fast_clss_dom:
+  \<open>(RETURN o isasat_fast_clss, RETURN o isasat_fast_clss_dom) \<in>
+      \<langle>Id\<rangle>clauses_l_fmat \<rightarrow>\<^sub>f \<langle>bool_rel\<rangle>nres_rel\<close>
+  apply (intro frefI nres_relI)
+  apply (auto simp:  clauses_ll_assn_def list_fmap_rel_def isasat_fast_clss_dom_def
+      isasat_fast_clss_def)
+  apply (subst (asm)(4) eq_commute)
+  apply auto
+  apply (case_tac \<open>dom_m y\<close>)
+   apply (auto simp: uint_max_def)
+  done
+
+definition (in -) isasat_fast_code :: \<open>twl_st_wll_trail_fast \<Rightarrow> bool\<close> where
+  \<open>isasat_fast_code = (\<lambda>(M', (N', n), _). n < uint32_max)\<close>
+
+
+lemma (in -)isasat_fast_clss_hnr[sepref_fr_rules]:
+  \<open>(return o (\<lambda>(N, n). n \<le> uint32_max), RETURN o isasat_fast_clss) \<in>
+       (arlO_assn clause_ll_assn)\<^sup>k \<rightarrow>\<^sub>a bool_assn\<close>
+  apply sepref_to_hoare
+  apply (sep_auto simp: isasat_fast_clss_def
+      isasat_fast2_def isasat_fast_code_def clauses_ll_assn_def
+      hr_comp_def list_fmap_rel_def arlO_assn_def arl_assn_def
+      is_array_list_def dest: heap_list_add_same_length
+      elim!: mod_starE)
+  done
+
+lemma isasat_fast_clss_dom_hnr [sepref_fr_rules]:
+\<open>((return \<circ>\<circ> case_prod) (\<lambda>N n. n \<le> uint_max),
+     RETURN \<circ> isasat_fast_clss_dom)
+    \<in> (clauses_ll_assn)\<^sup>k \<rightarrow>\<^sub>a bool_assn\<close>
+  using isasat_fast_clss_hnr[FCOMP isasat_fast_clss_dom] unfolding clauses_ll_assn_def[symmetric]
+  .
+
+lemma (in -)isasat_fast2_alt_def:
+  \<open>isasat_fast2 = (\<lambda>(M,N,_). isasat_fast_clss_dom N)\<close>
+  by (auto simp: isasat_fast2_def isasat_fast_clss_dom_def)
+
+
+context isasat_input_bounded_nempty
+begin
+
+declare isasat_fast_slow_code.refine[sepref_fr_rules]
+
+sepref_register isasat_fast2
+sepref_thm isasat_fast2_code
+  is \<open>RETURN o isasat_fast2\<close>
+  :: \<open>isasat_fast_assn\<^sup>k \<rightarrow>\<^sub>a bool_assn\<close>
+  supply [[goals_limit=1]]
+  unfolding isasat_fast2_alt_def isasat_fast_assn_def
+  by sepref
+
+concrete_definition (in -) isasat_fast2_code
+  uses isasat_input_bounded_nempty.isasat_fast2_code.refine_raw
+  is \<open>(?f, _) \<in> _\<close>
+
+prepare_code_thms (in -) isasat_fast2_code_def
+
+lemmas isasat_fast2_code[sepref_fr_rules] =
+   isasat_fast2_code.refine[OF isasat_input_bounded_nempty_axioms]
+
+sepref_register cdcl_twl_stgy_prog_wl_D_heur
+
+definition (in isasat_input_ops) cdcl_twl_stgy_prog_break_wl_D_heur_break
+   :: \<open>twl_st_wl_heur \<Rightarrow> twl_st_wl_heur nres\<close>
+where
+  \<open>cdcl_twl_stgy_prog_break_wl_D_heur_break S\<^sub>0 =
+  do {
+    (b, brk, T) \<leftarrow> WHILE\<^sub>T\<^bsup>\<lambda>(b, brk, S). (b \<longrightarrow> isasat_fast S)\<^esup>
+        (\<lambda>(b, brk, _). b \<and> \<not>brk)
+        (\<lambda>(b, brk, S).
+        do {
+          ASSERT b;
+          T \<leftarrow> unit_propagation_outer_loop_wl_D_heur S;
+          ASSERT(isasat_fast T);
+          (brk, T) \<leftarrow> cdcl_twl_o_prog_wl_D_heur T;
+          b \<leftarrow> RETURN (isasat_fast2 T);
+          RETURN(b, brk, T)
+        })
+        (True, False, S\<^sub>0);
+    if brk then (isasat_fast_slow T)
+    else do {
+         T \<leftarrow> isasat_fast_slow T;
+         cdcl_twl_stgy_prog_wl_D_heur T}
+  }\<close>
+
+sepref_register isasat_fast_slow
 sepref_thm cdcl_twl_stgy_prog_wl_D_fast_code
-  is \<open>PR_CONST cdcl_twl_stgy_prog_wl_D_heur\<close>
-  :: \<open>[isasat_fast]\<^sub>a isasat_fast_assn\<^sup>d \<rightarrow> isasat_fast_assn\<close>
-  unfolding cdcl_twl_stgy_prog_wl_D_heur_def PR_CONST_def
-  supply [[goals_limit = 1]]
-apply sepref_dbg_keep
-      apply sepref_dbg_trans_keep
-           apply sepref_dbg_trans_step_keep
-           apply sepref_dbg_side_unfold apply (auto simp: )[]
+  is \<open>PR_CONST cdcl_twl_stgy_prog_break_wl_D_heur_break\<close>
+  :: \<open>[isasat_fast]\<^sub>a isasat_fast_assn\<^sup>d \<rightarrow> isasat_assn\<close>
+  unfolding cdcl_twl_stgy_prog_break_wl_D_heur_break_def PR_CONST_def
+  supply [[goals_limit = 1]] isasat_input_bounded_nempty_axioms[intro]
   by sepref
 
 concrete_definition (in -) cdcl_twl_stgy_prog_wl_D_fast_code
@@ -597,7 +692,11 @@ lemmas cdcl_twl_stgy_prog_wl_D_fast_code[sepref_fr_rules] =
 
 end
 
+export_code cdcl_twl_stgy_prog_wl_D_fast_code in SML_imp module_name SAT_Solver
+  file "code/CDCL_Cached_Array_Trail_Fast.sml"
+
 export_code cdcl_twl_stgy_prog_wl_D_code in SML_imp module_name SAT_Solver
   file "code/CDCL_Cached_Array_Trail.sml"
+
 
 end
